src/proofs/Soundness.v
@@ -1,0 +1,55 @@
+(*Here we give the definition of soundness for transformations
+  in the errState monad: if the initial state if wf, then if the resulting
+  task(s) is/are valid, so is the initial one.*)
+From Proofs Require Import Task.
+Require Import Relations ErrStateHoare StateInvar.
+Require Import TaskDefs TransDefs.
+
+(*Version for single tarns (not list)*)
+(*NOTE: here, we do not require that the output is wf. We can prove that separately*)
+Definition trans_errst_sound (trans: trans_errst task) : Prop :=
+  forall (t: task),
+  (*put typing in precondition, some may be ill-defined without typing (though should just
+    be error which is OK because partial correctness)*)
+  errst_spec (fun s => st_wf t s /\ typed_task t) (trans t)
+    (fun (s1: full_st) (r: task) (s2: full_st) =>
+      valid_task r ->
+      valid_task t).
+
+(*Version for lists*)
+Definition trans_errst_list_sound (trans: trans_errst (list task)) : Prop :=
+  forall (t: task),
+  errst_spec (fun s => st_wf t s) (trans t)
+    (fun (s1: full_st) (r: list task) (s2: full_st) =>
+      Forall valid_task r ->
+      valid_task t).
+
+(*This definition is not terribly useful. Instead, we want to show
+  that the transformation relates to a stateless one in the core language
+  that is sound. We show that this condition implies soundness*)
+
+
+(*TODO: maybe I don't actually need var alpha for funpred_def -
+  my [open_ls_defn] is stateless, so we should never actually change
+  If I change this, should be easy I believe*)
+
+
+(*Here, just prove that related inputs -> related outputs, purely syntactic reasoning*)
+Lemma prove_trans_errst_sound (trans: trans_errst task) (tr1: Task.task -> Task.task):
+  sound_trans (single_trans tr1) ->
+  (forall tsk1 tsk2,
+    errst_spec (fun s => st_wf tsk1 s /\ task_related tsk1 tsk2) (trans tsk1)
+      (fun _ r _ => task_related r (tr1 tsk2))) ->
+  trans_errst_sound trans.
+Proof.
+  unfold sound_trans, TaskGen.sound_trans . intros Htrans Hrel.
+  unfold trans_errst_sound.
+  intros t.
+  (*Idea: look at [eval_task] t, know in precondition it (t1) is well-typed,
+    and know that [task_related t t1], so 
+    then, have precondition of Hrel, then know task_related r (tr1 t1),
+    use trans to know that t1 is valid, then use task_valid result to combine*)
+Admitted.
+
+
+  
